show annotated are logically equivalent to unannotated

theories/paris/examples/b_tree_adt.v
@@ -1170,11 +1170,22 @@ Section b_tree_adt.
       let: "t" := !"pt" in
       optimized_sampler_annotated_prog (max_child_num' := max_child_num') "t" #().
 
+  Definition opt_sampler_prog' : val :=
+    λ: "pt",
+      let: "t" := !"pt" in
+      optimized_sampler_prog (max_child_num' := max_child_num') "t" #().
+
   Definition naive_sampler_annotated_prog' : val :=
     λ: "pt",
        let: "t" := !"pt" in
        let: "rt" := build_ranked "t" in
        naive_sampler_annotated_prog "rt" #().
+
+  Definition naive_sampler_prog' : val :=
+    λ: "pt",
+       let: "t" := !"pt" in
+       let: "rt" := build_ranked "t" in
+       naive_sampler_prog "rt" #().
 
   Local Close Scope R.
 
@@ -1182,11 +1193,17 @@ Section b_tree_adt.
      creating a tree, second is inserting, and third is sampling *)
   Definition btreeτ : type := ∃: (TInt → #0) * (#0 * TInt → TUnit) * (#0 → TInt).
 
+  Definition opt_btree_pack : val :=
+    (init_tree, insert_tree, opt_sampler_prog').
+
   Definition opt_annotated_btree_pack : val :=
     (init_tree, insert_tree, opt_sampler_annotated_prog').
 
   Definition intermediate_btree_pack : val :=
     (init_tree, insert_tree, intermediate_sampler_prog').
+
+  Definition naive_btree_pack : val :=
+    (init_tree, insert_tree, naive_sampler_prog').
 
   Definition naive_annotated_btree_pack : val :=
     (init_tree, insert_tree, naive_sampler_annotated_prog').
@@ -1240,6 +1257,98 @@ Section b_tree_adt.
     iMod ("Hclo" with "[Hb1 Hb2 $Hna $Hforall']").
     { iNext. iExists _, _. iSplitL "Hb1"; iExists _; iFrame. }
     iModIntro. iExists _, _; iFrame. eauto.
+  Qed.
+
+  (* TODO: there's a lot of redundant boiler plate in several of these *)
+
+  Lemma opt_annotated_refines_opt Δ :
+    ⊢ REL opt_annotated_btree_pack  << opt_btree_pack : interp btreeτ Δ.
+  Proof.
+    iApply (refines_pack R).
+    rewrite refines_eq /refines_def. iIntros (K ε) "HK Hown Heps %Hlt".
+    wp_pures.
+    iModIntro. iExists _; iFrame. iSplit; first eauto. simpl.
+    iExists _, _, _, _.
+    iSplit; first eauto.
+    iSplit; first eauto.
+    clear Δ K ε Hlt.
+    iSplit; first (iExists _, _, _, _; iSplit; first eauto; iSplit; first eauto; iSplit).
+    - iApply init_tree_self_lrel.
+    - iApply insert_tree_self_lrel.
+    - iIntros (vv1 vv2) "!>".
+      iIntros "HR".
+      iDestruct "HR" as (p1 p2) "(->&->&Hinv)".
+      iApply (refines_na_inv with "[$Hinv]"); first done.
+      iIntros "(Hbtree&Hclo)".
+      rewrite /opt_sampler_prog'.
+      rewrite /opt_sampler_annotated_prog'.
+      rel_pures_l. rel_pures_r.
+      rewrite refines_eq /refines_def.
+      iIntros (K ε) "HK Hna Heps %Hlt".
+      wp_pures.
+      iDestruct "Hbtree" as (???) "(%Hforall&Hb1&Hb2)".
+      iDestruct "Hb1" as (?) "Hb1".
+      iDestruct "Hb2" as (?) "Hb2".
+
+      iDestruct "Hb1" as "(%His_tree&Hp1&Hrel1)".
+      iDestruct "Hb2" as "(%&Hp2&Hrel2)".
+      iApply wp_fupd.
+      wp_load. wp_pures.
+      tp_load. tp_pures.
+      iMod (ec_zero) as "Hz".
+      wp_apply (optimized_annotated_optimized_refinement with "[$Hrel1 $Hrel2 $Hz $HK]"); eauto.
+      iIntros (?) "(HK&%Helem&Hrel1&Hrel2)". iMod ("Hclo" with "[Hp1 Hp2 $Hna Hrel1 Hrel2]").
+      { iNext. rewrite /btree_inv. iExists _, _, _.
+        iFrame "%". iSplitL "Hp1 Hrel1"; iExists _; iFrame; eauto. }
+      iModIntro. iExists _, _. iFrame. iSplit; first done.
+      iPureIntro.
+      eapply Forall_forall in Hforall; last eauto.
+      destruct Hforall as (n&->). naive_solver.
+  Qed.
+
+  Lemma opt_refines_opt_annotated Δ :
+    ⊢ REL opt_btree_pack  << opt_annotated_btree_pack : interp btreeτ Δ.
+  Proof.
+    iApply (refines_pack R).
+    rewrite refines_eq /refines_def. iIntros (K ε) "HK Hown Heps %Hlt".
+    wp_pures.
+    iModIntro. iExists _; iFrame. iSplit; first eauto. simpl.
+    iExists _, _, _, _.
+    iSplit; first eauto.
+    iSplit; first eauto.
+    clear Δ K ε Hlt.
+    iSplit; first (iExists _, _, _, _; iSplit; first eauto; iSplit; first eauto; iSplit).
+    - iApply init_tree_self_lrel.
+    - iApply insert_tree_self_lrel.
+    - iIntros (vv1 vv2) "!>".
+      iIntros "HR".
+      iDestruct "HR" as (p1 p2) "(->&->&Hinv)".
+      iApply (refines_na_inv with "[$Hinv]"); first done.
+      iIntros "(Hbtree&Hclo)".
+      rewrite /opt_sampler_prog'.
+      rewrite /opt_sampler_annotated_prog'.
+      rel_pures_l. rel_pures_r.
+      rewrite refines_eq /refines_def.
+      iIntros (K ε) "HK Hna Heps %Hlt".
+      wp_pures.
+      iDestruct "Hbtree" as (???) "(%Hforall&Hb1&Hb2)".
+      iDestruct "Hb1" as (?) "Hb1".
+      iDestruct "Hb2" as (?) "Hb2".
+
+      iDestruct "Hb1" as "(%His_tree&Hp1&Hrel1)".
+      iDestruct "Hb2" as "(%&Hp2&Hrel2)".
+      iApply wp_fupd.
+      wp_load. wp_pures.
+      tp_load. tp_pures.
+      iMod (ec_zero) as "Hz".
+      wp_apply (annotated_optimized_optimized_refinement with "[$Hrel1 $Hrel2 $Hz $HK]"); eauto.
+      iIntros (?) "(HK&%Helem&Hrel1&Hrel2)". iMod ("Hclo" with "[Hp1 Hp2 $Hna Hrel1 Hrel2]").
+      { iNext. rewrite /btree_inv. iExists _, _, _.
+        iFrame "%". iSplitL "Hp1 Hrel1"; iExists _; iFrame; eauto. }
+      iModIntro. iExists _, _. iFrame. iSplit; first done.
+      iPureIntro.
+      eapply Forall_forall in Hforall; last eauto.
+      destruct Hforall as (n&->). naive_solver.
   Qed.
 
   Lemma intermediate_refines_opt_annotated Δ :
@@ -1453,6 +1562,118 @@ Section b_tree_adt.
       iMod (ec_zero) as "Hz".
       wp_apply (intermediate_annotated_naive_refinement with "[$Hrel1_ranked $Hrel2 $HK $Hz]"); eauto.
       iIntros (?) "(HK&%Helem&Hrel2&Hrel1_ranked)". iMod ("Hclo" with "[Hp1 Hp2 $Hna Hrel1 Hrel2]").
+      { iNext. rewrite /btree_inv. iExists _, _, _.
+        iFrame "%". iSplitR "Hp1 Hrel1"; iExists _; iFrame; eauto. }
+      iModIntro. iExists _, _. iFrame. iSplit; first by (iPureIntro; nra).
+      iPureIntro.
+      eapply Forall_forall in Hforall; last eauto.
+      destruct Hforall as (n&->). naive_solver.
+  Qed.
+
+  Lemma naive_refines_naive_annotated Δ :
+    ⊢ REL naive_btree_pack  << naive_annotated_btree_pack : interp btreeτ Δ.
+  Proof.
+    iApply (refines_pack R).
+    rewrite refines_eq /refines_def. iIntros (K ε) "HK Hown Heps %Hlt".
+    wp_pures.
+    iModIntro. iExists _; iFrame. iSplit; first eauto. simpl.
+    iExists _, _, _, _.
+    iSplit; first eauto.
+    iSplit; first eauto.
+    clear Δ K ε Hlt.
+    (* Break up the nested pair interpretation on the left so
+       that we get a flat hierarchy of 3 goals for each component of the 3 tuple *)
+    iSplit; first (iExists _, _, _, _; iSplit; first eauto; iSplit; first eauto; iSplit).
+    - iApply init_tree_self_lrel.
+    - iApply insert_tree_self_lrel.
+    - iIntros (vv1 vv2) "!>".
+      iIntros "HR".
+      iDestruct "HR" as (p1 p2) "(->&->&Hinv)".
+      iApply (refines_na_inv with "[$Hinv]"); first done.
+      iIntros "(Hbtree&Hclo)".
+      rewrite /naive_sampler_prog'.
+      rewrite /naive_sampler_annotated_prog'.
+      rel_pures_l. rel_pures_r.
+      rewrite refines_eq /refines_def.
+      iIntros (K ε) "HK Hna Heps %Hlt".
+      iDestruct "Hbtree" as (???) "(%Hforall&Hb1&Hb2)".
+      iDestruct "Hb1" as (?) "Hb1".
+      iDestruct "Hb2" as (?) "Hb2".
+
+      iDestruct "Hb2" as "(%His_tree&Hp1&Hrel1)".
+      iDestruct "Hb1" as "(%&Hp2&Hrel2)".
+      iApply wp_fupd.
+      wp_load. wp_pures.
+      tp_load. tp_pures.
+
+      tp_bind (build_ranked _).
+      iMod (spec_build_ranked with "[//] Hrel1 HK") as (treev') "(HK&Hrel1&Hrel1_ranked)".
+      simpl.
+      tp_pures.
+
+      wp_apply (wp_build_ranked with "[$Hrel2]"); first eauto.
+      iIntros (?) "(Hrel2&Hrel2_ranked)".
+      wp_pures.
+
+      iMod (ec_zero) as "Hz".
+      wp_apply (naive_annotated_naive_refinement with "[$Hrel1_ranked $Hrel2_ranked $HK $Hz]"); eauto.
+      iIntros (?) "(HK&%Helem&Hrel2_ranked&Hrel1_ranked)". iMod ("Hclo" with "[Hp1 Hp2 $Hna Hrel1 Hrel2]").
+      { iNext. rewrite /btree_inv. iExists _, _, _.
+        iFrame "%". iSplitR "Hp1 Hrel1"; iExists _; iFrame; eauto. }
+      iModIntro. iExists _, _. iFrame. iSplit; first by (iPureIntro; nra).
+      iPureIntro.
+      eapply Forall_forall in Hforall; last eauto.
+      destruct Hforall as (n&->). naive_solver.
+  Qed.
+
+  Lemma naive_annotated_refines_naive Δ :
+    ⊢ REL naive_annotated_btree_pack  << naive_btree_pack : interp btreeτ Δ.
+  Proof.
+    iApply (refines_pack R).
+    rewrite refines_eq /refines_def. iIntros (K ε) "HK Hown Heps %Hlt".
+    wp_pures.
+    iModIntro. iExists _; iFrame. iSplit; first eauto. simpl.
+    iExists _, _, _, _.
+    iSplit; first eauto.
+    iSplit; first eauto.
+    clear Δ K ε Hlt.
+    (* Break up the nested pair interpretation on the left so
+       that we get a flat hierarchy of 3 goals for each component of the 3 tuple *)
+    iSplit; first (iExists _, _, _, _; iSplit; first eauto; iSplit; first eauto; iSplit).
+    - iApply init_tree_self_lrel.
+    - iApply insert_tree_self_lrel.
+    - iIntros (vv1 vv2) "!>".
+      iIntros "HR".
+      iDestruct "HR" as (p1 p2) "(->&->&Hinv)".
+      iApply (refines_na_inv with "[$Hinv]"); first done.
+      iIntros "(Hbtree&Hclo)".
+      rewrite /naive_sampler_prog'.
+      rewrite /naive_sampler_annotated_prog'.
+      rel_pures_l. rel_pures_r.
+      rewrite refines_eq /refines_def.
+      iIntros (K ε) "HK Hna Heps %Hlt".
+      iDestruct "Hbtree" as (???) "(%Hforall&Hb1&Hb2)".
+      iDestruct "Hb1" as (?) "Hb1".
+      iDestruct "Hb2" as (?) "Hb2".
+
+      iDestruct "Hb2" as "(%His_tree&Hp1&Hrel1)".
+      iDestruct "Hb1" as "(%&Hp2&Hrel2)".
+      iApply wp_fupd.
+      wp_load. wp_pures.
+      tp_load. tp_pures.
+
+      tp_bind (build_ranked _).
+      iMod (spec_build_ranked with "[//] Hrel1 HK") as (treev') "(HK&Hrel1&Hrel1_ranked)".
+      simpl.
+      tp_pures.
+
+      wp_apply (wp_build_ranked with "[$Hrel2]"); first eauto.
+      iIntros (?) "(Hrel2&Hrel2_ranked)".
+      wp_pures.
+
+      iMod (ec_zero) as "Hz".
+      wp_apply (annotated_naive_naive_refinement with "[$Hrel1_ranked $Hrel2_ranked $HK $Hz]"); eauto.
+      iIntros (?) "(HK&%Helem&Hrel2_ranked&Hrel1_ranked)". iMod ("Hclo" with "[Hp1 Hp2 $Hna Hrel1 Hrel2]").
       { iNext. rewrite /btree_inv. iExists _, _, _.
         iFrame "%". iSplitR "Hp1 Hrel1"; iExists _; iFrame; eauto. }
       iModIntro. iExists _, _. iFrame. iSplit; first by (iPureIntro; nra).
